\section{Insights and Algorithms}

\subsection{Exercises}

\subsubsection{Exercise 3.1}
Assume $f(n) = 2^{n} - 1$. Then $f(n + 1) = 2^{n + 1} - 2 + 1 = 2^{n + 1} - 1$.

\subsubsection{Exercise 3.2}
We have that
\begin{align*}
        (QQ^* )_{ab} &= \frac{1}{n}\sum_{k = 0}^{n - 1} w_n^{ak} \bar{w_n^{kb}} \\
                     &= \frac{1}{n}\sum_{k = 0}^{n - 1} w_n^{k(i - j)}\\
\end{align*}
If $i = j$, then $(QQ^*)_{ab} = 1$. Otherwise, since $w_n^{(i - j)}$ is a root of unity,
\begin{align*}
        (QQ^*)_{ab} &= w_n^{i - j} (QQ^*)_{ab} \implies (1 - w_n^{i - j}) (QQ^*)_{ab} = 0 \implies
        (QQ^*)_{ab} = 0
\end{align*}
And we have that $Q^* = Q^{-1}$ as desired.
